New serialize_top interface

systems/Disk.v
@@ -10,15 +10,15 @@ Section Disk.
   Context {orig_failure_params : FailureParams orig_multi_params}.
   Context {data_serializer : Serializer data}.
 
-  Definition init_disk h := serialize_top serialize (init_handlers h).
+  Definition init_disk h := serialize_top (serialize (init_handlers h)).
   
   Definition disk_net_handlers dst src m st :=
     let '(out, data, ps) := net_handlers dst src m st in
-    (serialize_top serialize data, out, data, ps).
+    (serialize_top (serialize data), out, data, ps).
 
   Definition disk_input_handlers h inp st :=
     let '(out, data, ps) := input_handlers h inp st in
-    (serialize_top serialize data, out, data, ps).
+    (serialize_top (serialize data), out, data, ps).
 
   Instance disk_base_params : BaseParams :=
     {
